Add Coq syntax for MIR

coq/MIRSyntax.v
@@ -1,7 +1,4 @@
-From Coq Require Import Strings.String.
-From Coq Require Import ZArith.
-From Coq Require Import List.
-From Coq Require Import Bool.Bool.
+From Coq Require Import ZArith List String Bool.
 
 Import ListNotations.
 Open Scope string_scope.
@@ -9,61 +6,47 @@ Open Scope Z_scope.
 
 Module MIR.
 
-(** * Core MIR types *)
+(** * Week-1 MIR core syntax *)
 
 Inductive mir_ty :=
 | TyI32
+| TyU32
 | TyF32
-| TyU64
+| TyU64 (* pointer payload *)
 | TyBool.
 
-Inductive binop :=
-| BAdd
-| BSub
-| BMul
-| BDiv.
-
-Inductive expr :=
-| EConstInt (n : Z)
-| EConstFloat (bits : Z) (** Raw IEEE754 bits for now. *)
-| EVar (x : string)
-| EBinOp (op : binop) (lhs rhs : expr)
-| EPtrAdd (base : expr) (offset : expr).
-
-Inductive stmt :=
-| SAssign (dst : string) (rhs : expr)
-| SLoad (dst : string) (ptr : expr) (ty : mir_ty)
-| SStore (ptr : expr) (rhs : expr) (ty : mir_ty)
-| SAtomicLoadAcquire (dst : string) (ptr : expr) (ty : mir_ty)
-| SAtomicStoreRelease (ptr : expr) (rhs : expr) (ty : mir_ty)
-| SIf (cond : expr) (then_branch : list stmt) (else_branch : list stmt)
-| SLoop (body : list stmt)
-| SContinueLoop (body : list stmt)
-| SBreak
-| SBarrier.
-
-Definition block := list stmt.
-
-Record prog := {
-  prog_body : block
-}.
-
-Inductive value :=
-| VInt (n : Z)
-| VFloat (bits : Z)
-| VPtr (addr : Z)
+Inductive val :=
+| VI32 (z : Z)
+| VU32 (z : Z)
+| VF32 (bits : Z)
+| VU64 (addr : Z)
 | VBool (b : bool).
 
-Inductive event_mir :=
-| EvAssign (dst : string) (val : value)
-| EvLoad (ty : mir_ty) (addr : Z) (val : value)
-| EvStore (ty : mir_ty) (addr : Z) (val : value)
-| EvAtomicLoadAcquire (ty : mir_ty) (addr : Z) (val : value)
-| EvAtomicStoreRelease (ty : mir_ty) (addr : Z) (val : value)
-| EvBarrier
-| EvNop.
+Definition var := string.
+Definition addr := Z.
 
-Definition block_append (b rest : block) : block := b ++ rest.
-Definition singleton (s : stmt) : block := s :: nil.
+Inductive expr :=
+| EVal (v : val)
+| EVar (x : var)
+| EAdd (lhs rhs : expr)
+| EMul (lhs rhs : expr)
+| EPtrAdd (base ofs : expr).
+
+Inductive stmt :=
+| SAssign (x : var) (rhs : expr)
+| SLoad (x : var) (ptr : expr) (ty : mir_ty)
+| SStore (ptr : expr) (rhs : expr) (ty : mir_ty)
+| SAtomicLoadAcquire (x : var) (ptr : expr) (ty : mir_ty)
+| SAtomicStoreRelease (ptr : expr) (rhs : expr) (ty : mir_ty)
+| SBarrier
+| SIf (cond : expr) (then_branch else_branch : list stmt)
+| SSeq (body : list stmt).
+
+Inductive event_mir :=
+| EvLoad (ty : mir_ty) (addr : addr) (v : val)
+| EvStore (ty : mir_ty) (addr : addr) (v : val)
+| EvAtomicLoadAcquire (ty : mir_ty) (addr : addr) (v : val)
+| EvAtomicStoreRelease (ty : mir_ty) (addr : addr) (v : val)
+| EvBarrier.
 
 End MIR.
