coq/PTXImports.v
@@ -6,7 +6,13 @@ Require Import MIRSyntax.
 Module PTX.
 
 Inductive scope :=
-| ScopeCTA.
+| ScopeCTA
+| ScopeGPU
+| ScopeSYS.
+
+Inductive mem_space :=
+| SpaceGlobal
+| SpaceShared.
 
 Inductive mem_sem :=
 | SemRelaxed
@@ -26,28 +32,37 @@ Inductive payload :=
 | PayloadU64 (addr : Z).
 
 Inductive event :=
-| EvLoad (sc : scope) (sem : mem_sem) (ty : mem_ty) (addr : Z) (val : payload)
-| EvStore (sc : scope) (sem : mem_sem) (ty : mem_ty) (addr : Z) (val : payload)
+| EvLoad (space : mem_space) (sem : mem_sem) (sc : option scope)
+         (ty : mem_ty) (addr : Z) (val : payload)
+| EvStore (space : mem_space) (sem : mem_sem) (sc : option scope)
+          (ty : mem_ty) (addr : Z) (val : payload)
 | EvBarrier (sc : scope).
 
 Definition scope_cta : scope := ScopeCTA.
+Definition scope_sys : scope := ScopeSYS.
+Definition scope_gpu : scope := ScopeGPU.
 Definition sem_relaxed : mem_sem := SemRelaxed.
 Definition sem_acquire : mem_sem := SemAcquire.
 Definition sem_release : mem_sem := SemRelease.
 
+Definition space_global : mem_space := SpaceGlobal.
+Definition space_shared : mem_space := SpaceShared.
+
 Definition mem_ty_of_mir (ty : MIR.mir_ty) : mem_ty :=
   match ty with
   | MIR.TyI32 => MemU32
+  | MIR.TyU32 => MemU32
   | MIR.TyF32 => MemF32
   | MIR.TyU64 => MemU64
   | MIR.TyBool => MemPred
   end.
 
-Definition payload_of_mir (ty : MIR.mir_ty) (v : MIR.value) : option payload :=
+Definition payload_of_mir (ty : MIR.mir_ty) (v : MIR.val) : option payload :=
   match ty, v with
-  | MIR.TyI32, MIR.VInt n => Some (PayloadU32 n)
-  | MIR.TyF32, MIR.VFloat bits => Some (PayloadF32 bits)
-  | MIR.TyU64, MIR.VPtr addr => Some (PayloadU64 addr)
+  | MIR.TyI32, MIR.VI32 n => Some (PayloadU32 n)
+  | MIR.TyU32, MIR.VU32 n => Some (PayloadU32 n)
+  | MIR.TyF32, MIR.VF32 bits => Some (PayloadF32 bits)
+  | MIR.TyU64, MIR.VU64 addr => Some (PayloadU64 addr)
   | MIR.TyBool, MIR.VBool b => Some (PayloadPred b)
   | _, _ => None
   end.
