coq/MIRTests.v
@@ -1,0 +1,59 @@
+From Coq Require Import ZArith List String Bool.
+
+Import ListNotations.
+Open Scope string_scope.
+Open Scope Z_scope.
+
+Require Import MIRSyntax.
+Require Import MIRSemantics.
+Require Import MIRRun.
+
+Module M := MIR.
+Module MS := MIRSemantics.
+Module MR := MIRRun.
+
+Fixpoint lookup_mem (k : M.addr) (ps : list (M.addr * M.val)) : option M.val :=
+  match ps with
+  | [] => None
+  | (a, v) :: ps' => if Z.eqb k a then Some v else lookup_mem k ps'
+  end.
+
+Definition mem_of_pairs (ps : list (M.addr * M.val)) : MS.mem :=
+  {| MS.mem_get := fun k => lookup_mem k ps |}.
+
+Definition extend_env (ρ : MS.env) (x : M.var) (v : M.val) : MS.env :=
+  MS.env_set ρ x v.
+
+Definition empty_env : MS.env := MS.empty_env.
+
+(* === Test 1: relaxed load followed by store === *)
+
+Definition prog_load_store : list M.stmt :=
+  [ M.SLoad "t" (M.EVal (M.VU64 1000)) M.TyF32
+  ; M.SStore (M.EVal (M.VU64 2000)) (M.EVar "t") M.TyF32
+  ].
+
+Definition μ_ls : MS.mem := mem_of_pairs [(1000, M.VF32 42%Z); (2000, M.VF32 0%Z)].
+Definition cfg_ls : MS.cfg := MS.mk_cfg prog_load_store empty_env μ_ls.
+
+Eval compute in (MR.run 10 cfg_ls).
+
+(* === Test 2: barrier emits exactly one event === *)
+
+Definition prog_barrier : list M.stmt := [M.SBarrier].
+Definition cfg_barrier : MS.cfg := MS.mk_cfg prog_barrier empty_env μ_ls.
+
+Eval compute in (MR.run 3 cfg_barrier).
+
+(* === Test 3: acquire/release flag round trip === *)
+
+Definition prog_acqrel : list M.stmt :=
+  [ M.SAtomicStoreRelease (M.EVal (M.VU64 3000)) (M.EVal (M.VU32 1)) M.TyU32
+  ; M.SAtomicLoadAcquire "f" (M.EVal (M.VU64 3000)) M.TyU32
+  ].
+
+Definition μ_flag : MS.mem := mem_of_pairs [(3000, M.VU32 0%Z)].
+Definition cfg_flag : MS.cfg := MS.mk_cfg prog_acqrel empty_env μ_flag.
+
+Eval compute in (MR.run 10 cfg_flag).
+
